### Step 1: Rewrite the second equation
The second equation is:

\[
\frac{y - 2}{x - 14} = \frac{-8x}{98y}
\]

Cross multiply to eliminate the fractions:

\[
(y - 2)(98y) = (x - 14)(-8x)
\]

Expand both sides:

\[
98y^2 - 196y = -8x^2 + 112x
\]

Rearrange into a standard form:

\[
8x^2 - 112x + 98y^2 - 196y = 0 \tag{3}
\]

### Step 2: Substitute \( y^2 \) from the ellipse equation
From the first equation:

\[
4x^2 + 49y^2 = 196
\]

Solve for \( y^2 \):

\[
y^2 = \frac{196 - 4x^2}{49} \tag{4}
\]

Substitute this \( y^2 \) expression into equation (3):

\[
8x^2 - 112x + 98\left(\frac{196 - 4x^2}{49}\right) - 196y = 0
\]

Simplify the \( 98 \cdot \frac{196 - 4x^2}{49} \) term:

\[
98 \cdot \frac{196 - 4x^2}{49} = 2(196 - 4x^2) = 392 - 8x^2
\]

Now the equation becomes:

\[
8x^2 - 112x + 392 - 8x^2 - 196y = 0
\]

Simplify:

\[
-112x + 392 - 196y = 0
\]

Solve for \( y \):

\[
196y = 392 - 112x
\]

\[
y = \frac{392 - 112x}{196} = 2 - \frac{4x}{7} \tag{5}
\]

### Step 3: Substitute \( y \) into the ellipse equation
Substitute \( y = 2 - \frac{4x}{7} \) into the ellipse equation \( 4x^2 + 49y^2 = 196 \):

\[
4x^2 + 49\left(2 - \frac{4x}{7}\right)^2 = 196
\]

Expand \( \left(2 - \frac{4x}{7}\right)^2 \):

\[
\left(2 - \frac{4x}{7}\right)^2 = 4 - \frac{16x}{7} + \frac{16x^2}{49}
\]

Substitute this into the equation:

\[
4x^2 + 49\left(4 - \frac{16x}{7} + \frac{16x^2}{49}\right) = 196
\]

Simplify the terms:

\[
4x^2 + 49(4) - 49\left(\frac{16x}{7}\right) + 49\left(\frac{16x^2}{49}\right) = 196
\]

\[
4x^2 + 196 - 112x + 16x^2 = 196
\]

Combine like terms:

\[
20x^2 - 112x + 196 = 196
\]

Simplify further:

\[
20x^2 - 112x = 0
\]

Factorize:

\[
4x(5x - 28) = 0
\]

### Step 4: Solve for \( x \)
From the factorization:

\[
4x = 0 \quad \text{or} \quad 5x - 28 = 0
\]

\[
x = 0 \quad \text{or} \quad x = \frac{28}{5} = 5.6
\]

### Step 5: Solve for \( y \)
Substitute each \( x \) value into \( y = 2 - \frac{4x}{7} \) (equation 5).

1. For \( x = 0 \):

\[
y = 2 - \frac{4(0)}{7} = 2
\]

2. For \( x = 5.6 \):

\[
y = 2 - \frac{4(5.6)}{7} = 2 - \frac{22.4}{7} = 2 - 3.2 = -1.2
\]

### Final Solution
The solutions are:

\[
(x, y) = (0, 2) \quad \text{and} \quad (x, y) = (5.6, -1.2)
\]
